\documentclass[a4paper]{article}

\usepackage{fullpage} % Package to use full page
\usepackage{parskip} % Package to tweak paragraph skipping
\usepackage{amsmath}
\usepackage{hyperref}
\usepackage{amsmath,amsfonts,amsthm} % Math packages
\usepackage{graphicx}
\usepackage{listings}
\usepackage{color}
\usepackage{float}
\definecolor{codegreen}{rgb}{0,0.6,0}
\definecolor{codegray}{rgb}{0.5,0.5,0.5}
\definecolor{codepurple}{rgb}{0.58,0,0.82}
\definecolor{backcolour}{rgb}{0.95,0.95,0.92}
\definecolor{brown}{rgb}{0.59, 0.29, 0.0}
\definecolor{beaublue}{rgb}{0.74, 0.83, 0.9}
\definecolor{orange}{rgb}{1.0, 0.5, 0.0}
\definecolor{darkslategray}{rgb}{0.18, 0.31, 0.31}

\lstdefinestyle{mystyle}{
	backgroundcolor=\color{white},   
	commentstyle=\color{codegreen},
	keywordstyle=\color{blue},
	identifierstyle=\color{brown},
	numberstyle=\tiny\color{codegray},
	stringstyle=\color{orange},
	basicstyle=\footnotesize,
	breakatwhitespace=false,         
	breaklines=true,                 
	captionpos=b,                    
	keepspaces=true,                 
	numbers=left,                    
	numbersep=5pt,                  
	showspaces=false,                
	showstringspaces=false,
	showtabs=false,                  
	tabsize=2
}
\lstset{style=mystyle}

\title{AMATH 567: Problem Set 7}
\author{Jithin D. George, No. 1622555}
\date{11/16/16}

\begin{document}

\maketitle
\begin{enumerate}
	
	\item
	\begin{enumerate}
		\item 
		\[
				\wp(z)=\frac{1}{z^2}+\sum_{j,k=-\infty}^\infty \left(\frac{1}{(z-j
					\omega_1-k \omega_2)^2}-\frac{1}{(j \omega_1+k \omega_2)^2}\right)		\]	
				Here, the term where both j and k are zero is removed.	                         
			\begin{center}             
			\begin{gather*}
		\wp(z+M \omega_1+N \omega_2)=\frac{1}{(z+M \omega_1+N \omega_2)^2}+\sum_{j,k=-\infty}^\infty \left(\frac{1}{(z+(M-j)
			\omega_1+(N-k) \omega_2)^2}-\frac{1}{(j \omega_1+k \omega_2)^2}\right)	
		\\= \\	
	\wp(z+M \omega_1)=\frac{1}{(z+M \omega_1)^2}+\sum_{j,k=-\infty}^\infty \left(\frac{1}{(z+(M-j)
		\omega_1-k \omega_2)^2} -\frac{1}{(j \omega_1+k \omega_2)^2}\right)	
		\\= \frac{1}{(z+M \omega_1)^2}+\sum_{j,k=-\infty}^\infty \left(\frac{1}{(z+(M-j)
			\omega_1-k \omega_2)^2} -\frac{1}{(z-j
			\omega_1-k \omega_2)^2}+\frac{1}{(z-j
			\omega_1-k \omega_2)^2}-\frac{1}{(j \omega_1+k \omega_2)^2}\right)	
		\\= \frac{1}{(z+M \omega_1)^2}+\\\underbrace{\sum_{j,k=-\infty}^\infty \left(\frac{1}{(z+(M-j)
			\omega_1-k \omega_2)^2} -\frac{1}{(z-j
			\omega_1-k \omega_2)^2}\right)}_\text{This is a telescoping series and hence not divergent}+\underbrace{\sum_{j,k=-\infty}^\infty \left(\frac{1}{(z-j
			\omega_1-k \omega_2)^2}-\frac{1}{(j \omega_1+k \omega_2)^2}\right)}_\text{This is the same type sequence as before and hence not divergent} 
	\\=	\frac{1}{(z+M \omega_1)^2}+\\\underbrace{\sum_{k=0,j-\infty, j\neq 0}^\infty \left(\frac{1}{(z+(M-j)
			\omega_1-k \omega_2)^2} -\frac{1}{(z-j
			\omega_1-k \omega_2)^2}\right)}_\text{if $k\neq0$, every term is cancelled by the Mth term after it} 	+\sum_{j,k=-\infty}^\infty \left(\frac{1}{(z-j
			\omega_1-k \omega_2)^2}-\frac{1}{(j \omega_1+k \omega_2)^2}\right)	
	\\=	\frac{1}{(z+M \omega_1)^2}+\sum_{j-\infty, j\neq 0}^\infty \left(\frac{1}{(z+(M-j)
			\omega_1)^2} -\frac{1}{(z-j
			\omega_1)^2}\right)	+\wp(z) - \frac{1}{z^2}		
	\\=	\frac{1}{(z+M \omega_1)^2}+ \left(\frac{1}{(z)^2} -\frac{1}{(z+M
		\omega_1)^2}\right)	+\wp(z) - \frac{1}{z^2}	
\\	=\wp(z)
								\end{gather*} 
						\end{center}
		
		\item
		\[	\wp(z)=\frac{1}{z^2}+\sum_{j,k=-\infty}^\infty \left(\frac{1}{(z-j
			\omega_1-k \omega_2)^2}-\frac{1}{(j \omega_1+k \omega_2)^2}\right)\]
		                         	\begin{center}             
		                         		\begin{gather*}
	\wp(z)	=\frac{1}{z^2}+ \frac{1}{(z- \omega_1)^2}+ \frac{1}{(z+ \omega_1)^2}+ \frac{1}{(z- \omega_2)^2}+ \frac{1}{(z+ \omega_2)^2}+ \frac{2}{( \omega_1)^2} + \frac{2}{(\omega_2)^2}
	 \\ +\sum_{j,k=1}^\infty \left(\frac{1}{(z-j
				\omega_1-k \omega_2)^2}-\frac{1}{(j \omega_1+k \omega_2)^2}\right)		+ \sum_{j,k=-1}^{-\infty} \left(\frac{1}{(z-j
		\omega_1-k \omega_2)^2}-\frac{1}{(j \omega_1+k \omega_2)^2}\right)		
		\\		=\frac{1}{z^2}+ \frac{1}{(z- \omega_1)^2}+ \frac{1}{(z+ \omega_1)^2}+ \frac{1}{(z- \omega_2)^2}+ \frac{1}{(z+ \omega_2)^2}+ \frac{2}{( \omega_1)^2} + \frac{2}{(\omega_2)^2}
		\\+\sum_{j,k=1}^\infty \left(\frac{1}{(z-j
			\omega_1-k \omega_2)^2}-\frac{1}{(j \omega_1+k \omega_2)^2}\right)		+ \sum_{j,k=1}^{\infty} \left(\frac{1}{(z+j
			\omega_1+k \omega_2)^2}-\frac{1}{(j \omega_1+k \omega_2)^2}\right)								\end{gather*} 
		\end{center}
			
		                         	\begin{center}             
                \begin{gather*}
   \wp(-z)		=\frac{1}{z^2}+ \frac{1}{(-z- \omega_1)^2}+ \frac{1}{(-z+ \omega_1)^2}+ \frac{1}{(-z- \omega_2)^2}+ \frac{1}{(-z+ \omega_2)^2}+ \frac{2}{( \omega_1)^2} \frac{2}{(\omega_2)^2}
		\\	+\sum_{j,k=1}^\infty \left(\frac{1}{(-z-j
				\omega_1-k \omega_2)^2}-\frac{1}{(j \omega_1+k \omega_2)^2}\right)	 \\	 + \sum_{j,k=1}^{\infty} \left(\frac{1}{(-z+j
				\omega_1+k \omega_2)^2}-\frac{1}{(j \omega_1+k \omega_2)^2}\right)		
		\\	=\frac{1}{z^2}+ \frac{1}{(z+ \omega_1)^2}+ \frac{1}{(z- \omega_1)^2}+ \frac{1}{(z+ \omega_2)^2}+ \frac{1}{(z- \omega_2)^2}+ \frac{2}{( \omega_1)^2} + \frac{2}{(\omega_2)^2}
		\\	+\sum_{j,k=1}^\infty \left(\frac{1}{(z+j
				\omega_1+k \omega_2)^2}-\frac{1}{(j \omega_1+k \omega_2)^2}\right)		+ \sum_{j,k=-1}^{\infty} \left(\frac{1}{(z-j
				\omega_1-k \omega_2)^2}-\frac{1}{(j \omega_1+k \omega_2)^2}\right)
		\\	=	   \wp(z)	
				\end{gather*} 
				\end{center}
	\item 
	$\wp(z)$ has a singularity at the origin. But
	\[ f(z) =\wp(z) - \frac{1}{z^2}	
	\] has no singularity around the origin and we can obtain a taylor series around the origin.
	\[ f'(z)= -2 \sum_{j,k=-\infty}^\infty \frac{1}{(z-j
		\omega_1-k \omega_2)^3} \]
		                         	\begin{center}             
		                         		\begin{gather*}
      f'(0)= -2  \sum_{j,k=-\infty}^\infty \frac{1}{(-j
		\omega_1-k \omega_2)^3} \\= -2 \left(\frac{1}{(\omega_1)^3}+ \frac{1}{(- \omega_1)^3}+ \frac{1}{( \omega_2)^3}+ \frac{1}{(- \omega_2)^3} 
		+\sum_{j,k=1}^\infty \frac{1}{(j
		\omega_1+k \omega_2)^3}	+ \sum_{j,k=1}^{\infty} \frac{1}{(-j
		\omega_1-k \omega_2)^3} \right)
	\\=0
	\end{gather*} 
	\end{center}
	Similarly, $f'''(z)=0$ and $f^{2n+1}(z)=0$ where n is a non-negative integer.	
	\[ f^{2n}(z) = (2n+1)! \sum_{j,k=-\infty}^\infty \frac{1}{(j
		\omega_1+k \omega_2)^{2n+2}} , f(0)=0  \]
	\[ \wp(z) = \frac{1}{z^2} + \sum_{n=1}^\infty \frac{f^{2n}}{2n!} z^{2n} \]	
		\[ \wp(z) = \frac{1}{z^2} + \alpha_0 +\alpha_2 z^2 + \alpha_4 z^4 ... \]
		\[ \alpha_0 = 0\]
		\[ \alpha_2 = 3 \sum_{j,k=-\infty}^\infty \frac{1}{(j
			\omega_1+k \omega_2)^{4}}\]
		\[ \alpha_4 = 5 \sum_{j,k=-\infty}^\infty \frac{1}{(j
			\omega_1+k \omega_2)^{6}}\]		
	\[ \wp'(z) = \frac{-2}{z^3} + \sum_{n=1}^\infty 2n \frac{f^{2n}}{2n!} z^{2n-1} \]
	\[
	\wp'(z)=-\frac{2}{z^3}+\beta_1 z+\beta_3 z^3+\ldots.
	\]

			\[ \beta_1 = 6 \sum_{j,k=-\infty}^\infty \frac{1}{(j
				\omega_1+k \omega_2)^{4}}\]
			\[ \beta_2 = 20 \sum_{j,k=-\infty}^\infty \frac{1}{(j
				\omega_1+k \omega_2)^{6}}\]	
	
\item
\[
(\wp')^2=a \wp^3+b \wp^2+c \wp+d,
\]
\[
(-\frac{2}{z^3}+\beta_1 z+\beta_3 z^3+\ldots)^2=a (\frac{1}{z^2}  +\alpha_2 z^2 ..)^3+b (\frac{1}{z^2}  +\alpha_2 z^2 ..)^2+c(\frac{1}{z^2}  +\alpha_2 z^2 ..) +d
\]
		                         	\begin{center}             
		                         		\begin{gather*}
(\frac{4}{z^6} -\frac{4\beta_1}{z^2} -4  \beta_3+\beta_1^2z^2+2\beta_1\beta_3 z^4 +\beta_3^2 z^6 ...)\\=a (\alpha_4^3 z^{12}+3 \alpha_4^2 \alpha_2 z^{10}+3 \alpha_4^2 z^6+3 \alpha_4 \alpha_2^2 z^8+6 \alpha_4 \alpha_2z^4+3 \alpha_4+\alpha_2^3 z^6+3 \alpha_2^2 z^2+\frac{3 \alpha_2}{z^2}+\frac{1}{z^6}..)\\+b (\alpha_4^2 z^6+2 \alpha_4 \alpha_2 z^5+2 \alpha_4 z+\alpha_2^2 z^4+2 \alpha_2+\frac{1}{z^4} ..)+c(\frac{1}{z^2}  +\alpha_2 z^2 ..) +d 	\end{gather*} 
\end{center}
Equating the coefficients of $z^{-6}$,
\[a=4\]
Since the first term on the right side and the left side does not have a $z^{-4}$ term.
\[b=0\]
Equating the coefficients of $z^{-2}$,
\[c =-4\beta_1+a3\alpha_2= -4\beta_1+12\alpha_2 \]
Equating constants,
\[d= -4 \beta_3 +a3\alpha_4 = -4 \beta_3 +12\alpha_4 \]




			
\end{enumerate} 
\item 
\begin {enumerate}
\item 
Substituting U(x) into the KdV equation
\[  U_t = 6UU_x +U_{xxx} \]
\[  0 = 6UU_x +U_{xxx} \]
On integration,
\[  C = 3U^2 +U_{xx} \]
Multiplying with $U_x$,
\[  CU_x = 3U^2U_x +U_{xx}U_x \]
Integrating,
\[ k+ CU = U^3  + \frac{U_x ^2}{2} \]
\[ U_x ^2= -2 U^3 +CU +k  \]
\item 
Substituting $U = U_0 \wp(x)$ (taking $x_0=0$),
\[U_0^2\wp_x^2= -2U_0^3\wp^3 +CU_0\wp+k\]
Substituting $(\wp')^2=a \wp^3+b \wp^2+c \wp+d $ ,
\[
U_0^2(a \wp^3+b \wp^2+c \wp+d)=-2U_0^3\wp^3 +CU_0\wp+k
\]
Equating coefficients of $\wp^3$,
\[a = -2U_0\]
\[U_0= -\frac{a}{2}=-2 \]


\end{enumerate} 
\item
\begin{enumerate}
\item
\[ -ln(\Gamma) = ln(z) + \gamma z + \sum_{n=1}^\infty \left(ln(\frac{n+z}{n}) -\frac{z}{n} \right) \]
\[ ln(\Gamma) = -ln(z) - \gamma z - \sum_{n=1}^\infty \left(ln(\frac{n+z}{n}) -\frac{z}{n} \right) \]
Differentiating,
\[ \frac{\Gamma'(z)}{\Gamma(z)} = -\frac{1}{z} - \gamma - \sum_{n=1}^\infty \left( \frac{1}{n}\frac{n}{n+z} -\frac{1}{n} \right) \]
\[ \frac{\Gamma'(z)}{\Gamma(z)} = -\frac{1}{z} - \gamma - \sum_{n=1}^\infty \left( \frac{1}{z+n} -\frac{1}{n} \right) \]
\item 
\[ \frac{\Gamma'(z)}{\Gamma(z)} = -\frac{1}{z} - \gamma - \sum_{n=1}^\infty \left( \frac{1}{z+n} -\frac{1}{n} \right) \]
		                         	\begin{center}             
		                         		\begin{gather*}
 \frac{\Gamma'(z+1)}{\Gamma(z+1)} = -\frac{1}{z+1} - \gamma - \sum_{n=1}^\infty \left( \frac{1}{z+1+n} -\frac{1}{n} \right)
			\\ = -\frac{1}{z+1} - \gamma - \sum_{1+n=2}^\infty \left( \frac{1}{z+1+n} -\frac{1}{n} \right)
			\\ = -\frac{1}{z+1} - \gamma - \sum_{j=2}^\infty \left( \frac{1}{z+j} -\frac{1}{j-1} \right)
			\\ =  - \gamma - \sum_{j=1}^\infty \left( \frac{1}{z+j} -\frac{1}{j} \right)
			\\ =  - \gamma - \sum_{n=1}^\infty \left( \frac{1}{z+n} -\frac{1}{n} \right)
			\\=\frac{\Gamma'(z)}{\Gamma(z)}  +\frac{1}{z}				                         			\end{gather*} 
		                         		\end{center}
		                         		
			\[ \frac{\Gamma'(z+1)}{\Gamma(z+1)} -\frac{\Gamma'(z)}{\Gamma(z)} -\frac{1}{z} =0 \]	
			Integrating,
			\[\ln(\Gamma(z+1))-\ln(\Gamma(z))-ln(z)=b	\] 	   
			\[\frac{\Gamma(z+1)}{\Gamma(z)} = Cz\]   
			\[   \Gamma(z+1)= Cz\Gamma(z) \]  
\item 
\[\lim_{z\to0} z\Gamma(z) = \lim_{z\to 0} \frac{1}{e^{\gamma z} \prod_{n=1}^{\infty} (1+ \frac{z}{n})e^{\frac{-z}{n}} } =1 \]
\[\lim_{z\to0}  \Gamma(z+1)= \lim_{z\to0}  Cz\Gamma(z) \]   
\[ \Gamma(1)=  C \]     
\item
Choosing C such that
 \[ \Gamma(1)=  1 \] 
 \[\frac{1}{e^{\gamma} \prod_{n=1}^{\infty} (1+ \frac{1}{n})e^{\frac{-1}{n}} } =1 \]
 \[e^{-\gamma}   =\prod_{n=1}^{\infty} (1+ \frac{1}{n})e^{\frac{-1}{n}} \]
 \item
    \[\prod_{n=1}^{\infty} (1+ \frac{1}{n})e^{\frac{-1}{n}}=\lim_{N\to \infty}\prod_{n=1}^{N} (1+ \frac{1}{n})e^{\frac{-1}{n}} = \lim_{N\to \infty}\frac{2}{1}\frac{3}{2}\frac{4}{3}..\frac{N+1}{N}e^{-S_N} = \lim_{N\to \infty}(N+1)e^{-S_N} \]     
    where \[S_N = 1+ \frac{1}{2}   + \frac{1}{3} +  ...   + \frac{1}{N}	\]	
     \[e^{-\gamma}   =\prod_{n=1}^{\infty} (1+ \frac{1}{n})e^{\frac{-1}{n}} \]
     \[ \gamma = -ln(\lim_{N\to \infty}(N+1)e^{-S_N})\]
     \[ \gamma =\lim_{N\to \infty} -ln((N+1)e^{-S_N}) =\lim_{N\to \infty}\sum_{k=1}^\infty \frac{1}{k} -ln(N+1)  \] 
\end{enumerate}
	\end{enumerate} 
\end{document}