\documentclass[a4paper]{article}

\usepackage{fullpage} % Package to use full page
\usepackage{parskip} % Package to tweak paragraph skipping
\usepackage{amsmath}
\usepackage{hyperref}
\usepackage{amsmath,amsfonts,amsthm} % Math packages
\usepackage{graphicx}
\usepackage{listings}
\usepackage{color}
\usepackage{float}
\definecolor{codegreen}{rgb}{0,0.6,0}
\definecolor{codegray}{rgb}{0.5,0.5,0.5}
\definecolor{codepurple}{rgb}{0.58,0,0.82}
\definecolor{backcolour}{rgb}{0.95,0.95,0.92}
\definecolor{brown}{rgb}{0.59, 0.29, 0.0}
\definecolor{beaublue}{rgb}{0.74, 0.83, 0.9}
\definecolor{orange}{rgb}{1.0, 0.5, 0.0}
\definecolor{darkslategray}{rgb}{0.18, 0.31, 0.31}


\lstdefinestyle{mystyle}{
	backgroundcolor=\color{white},   
	commentstyle=\color{codegreen},
	keywordstyle=\color{blue},
	identifierstyle=\color{brown},
	numberstyle=\tiny\color{codegray},
	stringstyle=\color{orange},
	basicstyle=\footnotesize,
	breakatwhitespace=false,         
	breaklines=true,                 
	captionpos=b,                    
	keepspaces=true,                 
	numbers=left,                    
	numbersep=5pt,                  
	showspaces=false,                
	showstringspaces=false,
	showtabs=false,                  
	tabsize=2
}
\lstset{style=mystyle}

\title{AMATH 567: Problem Set 8}
\author{Jithin D. George, No. 1622555}
\date{23/11/16}

\begin{document}

\maketitle
\begin{enumerate}
	
	\item
	\begin{enumerate}

\item 

		\[ f(z) = \frac{z^2+1}{z^2-a^2}=\frac{z^2+1}{(z-a)(z+a)}\]
	\begin{enumerate}
		
		\item 
		

		Since the singularities lie inside the unit circle as $a <1$,
		\[\frac{1}{2\pi i}\oint_C f(z) \,dz= Res_{z=-a}f(z)+Res_{z=a}f(z)\]
		\[=-\frac{a^2+1}{2a}+\frac{a^2+1}{2a} =0\]
			\item
			
			Taking the residue at infinity,
			\[\frac{1}{2\pi i}\oint_C f(z) \,dz= -Res_{z=\infty}f(z)=Res_{t=0}(\frac{1}{t^2})f(\frac{1}{t})\]
		\[	=Res_{t=0} (\frac{1}{t^2})\frac{\frac{1}{t^2}+1}{\frac{1}{t^2}-a^2}\]	
		\[=Res_{t=0} (\frac{1}{t^2})\frac{t^2+1}{1-a^2t^2}\]
		As it is a double pole at t=0,	 
		\[=\lim_{t \to 0} \frac{d}{dt}\left(\frac{t^2+1}{1-a^2t^2}\right)\]
		\[=\lim_{t \to 0} \left(\frac{2t(1-a^2t^2)+2a^2t(t^2+1)}{(1-a^2t^2)^2}\right)\]
		\[=0\]
		
	
\end{enumerate} 
\item 
\[ f(z) = \frac{1}{z}+\frac{1}{z^3}\]
\begin{enumerate}
	
	\item 
	
	
	The singularity is at 0,
	\[\frac{1}{2\pi i}\oint_C f(z) \,dz= Res_{z=0}f(z)=1\]
	\item
	
	Taking the residue at infinity,
	\[\lim_{z\to\infty} f(z)= \frac{1}{\infty}+\frac{1}{\infty} =0 \]
	\[\frac{1}{2\pi i}\oint_C f(z) \,dz= Res_{z=\infty}f(z)= \lim_{z\to\infty} zf(z)= 1 \]
	
\end{enumerate}
\item 
\[ f(z) = z^2e^{-\frac{1}{z}} = z^2 -z+\frac{1}{2}-\frac{1}{3!z}+\frac{1}{4!z^2} + \ldots \]
\begin{enumerate}
	
	\item 
	
	
	The singularity is at 0,
	\[\frac{1}{2\pi i}\oint_C f(z) \,dz= Res_{z=0}f(z)=-\frac{1}{3!}\]
	\item
	
	Taking the residue at infinity,
	\[\frac{1}{2\pi i}\oint_C f(z) \,dz= Res_{z=\infty}f(z)=Res_{t=0}(\frac{1}{t^2})f(\frac{1}{t}) \]
	\[ =Res_{t=0}(\frac{1}{t^2})(\frac{1}{t^2} -\frac{1}{t}+\frac{1}{2}-\frac{t}{3!}+\frac{t^2}{4!} + \ldots )\]
		\[ =Res_{t=0}(\frac{1}{t^4!} -\frac{1}{t^3}+\frac{1}{2t^2}-\frac{1}{3!t^2}+\frac{1}{4!} + \ldots )\]
		\[=-\frac{1}{3!}\]
	
\end{enumerate}  
\end{enumerate} 
\item
\[ \int_{0}^{\infty} \frac{dx}{(x^2+a^2)(x^2+b^2)}=\int_{0}^{\infty} \frac{dx}{(x+ia)(x-ia)(x+ib)(x-ib)}\] 
Consider the contour of a semicircle of radius R with its diameter going from -R to R on the real line. Let C be the contour as R goes to infinity. The singularities inside C are at ib and ia. $C_R$ is the arc going from 0 to $2\pi$.
\[f(z)=\frac{1}{(z+ia)(z-ia)(z+ib)(z-ib)}\]
\[\int_{C}f(z)dz = 2\pi i (Res_{z=ib}f(z) +Res_{z=ia}f(z)\]
\[\int_{C_R}f(z)dz +\int_{0}^{\infty}f(x)dx+\int_{-\infty}^{0} f(x) dx= 2\pi i (Res_{z=ib}f(z) +Res_{z=ia}f(z))\]
\[\underbrace{0}_\text{Theorem 4.2.1} +\int_{0}^{\infty}f(x)dx+\int_{-\infty}^{0}f(x)dx= 2\pi i (\frac{1}{(i(b+a))(i(b-a))(2ib))}-\frac{1}{(i(b+a))(i(b-a))(2ia))})\]
\[\int_{0}^{\infty}f(x)dx+\int_{-\infty}^{0}f(x)dx= 2\pi i (\frac{2i(a-b)}{(i(b+a))(i(a-b))(4ab))})= \frac{4\pi}{((b+a))(4ab))}\]
		                         	\begin{center}       
		                         		\begin{gather*}
\int_{0}^{\infty}f(x)dx+\int_{-\infty}^{0}f(x)dx=\int_{0}^{\infty}f(x)dx +\int_{\infty}^{0}\frac{e^{\pi i}}{(t^2+a^2)(t^2+b^2)}dt \\=\int_{0}^{\infty}f(x)dx -\int_{\infty}^{0}\frac{1}{(t^2+a^2)(t^2+b^2)}dt \\=\int_{0}^{\infty}f(x)dx +\int_{0}^{\infty}\frac{1}{(t^2+a^2)(t^2+b^2)}dt  \\=2 \int_{0}^{\infty}f(x)dx 
                       			\end{gather*} 
		                         		\end{center}
\[\int_{0}^{\infty}f(x)dx= \frac{\pi}{2((b+a))(ab))}\]	
When a=b,
\[f(z)=\frac{1}{(z+ia)^2(z-ia)^2}\]
\[2\int_{0}^{\infty}f(x)dx= 2\pi i (Res_{z=ia}f(z))\]
Since there is a double pole at ia,
\[2\int_{0}^{\infty}f(x)dx= 2\pi i\lim_{z\to ia} \frac{d}{dx}\frac{1}{(z+ia)^2}\]
\[\int_{0}^{\infty}f(x)dx= \pi i\lim_{z\to ia} \frac{-2}{(z+ia)^3}= \frac{\pi}{4a^3}\]

\item	
\[ \int_{-\infty}^{\infty} \frac{cos(kx) dx}{(x^2+a^2)(x^2+b^2)}=\int_{-\infty}^{\infty} \frac{cos(kx) dx}{(x+ia)(x-ia)(x+ib)(x-ib)}\]  
Consider the contour of a semicircle of radius R with its diameter going from -R to R on the real line. Let C be the contour as R goes to infinity. The singularities inside C are at ib and ia. $C_R$ is the arc going from 0 to $2\pi$.
\[p(z)=\frac{cos(kx) dx}{(x+ia)(x-ia)(x+ib)(x-ib)}\]
\[p(z)= Re(f(z))\]
\[f(z)=\frac{e^{ikz}}{(z+ia)(z-ia)(z+ib)(z-ib)}\]
\[	  	\int_{C_R}f(z)dz+\int_{-\infty}^{\infty}f(x)dx= 2\pi i (Res_{z=ia}f(z) +Res_{z=ib}f(z)\]
\[	  \underbrace{0}_\text{Jordan's Lemma}+\int_{-\infty}^{\infty}f(x)dx= 2\pi i (Res_{z=ia}f(z) +Res_{z=ib}f(z))\]
		                         	\begin{center}       
		                         		\begin{gather*}
	\int_{-\infty}^{\infty}f(x)dx= 2\pi i (\frac{e^{-ka}}{(2ia)i(a+b)i(a-b)}- \frac{e^{-kb}}{i(b+a)i(a-b)(2ib)}) 
	\\= \pi  (-\frac{e^{-ka}}{(a)(a+b)(a-b)}+ \frac{e^{-kb}}{(b+a)(a-b)(b)})
	%	\\= \pi  (-\frac{cosh(ka)}{(a)(a+b)(a-b)}+ %\frac{cosh(kb)}{(b+a)(a-b)(b)})
		\\= \pi  ( \frac{ae^{-kb}-be^{-ka}}{(b+a)(a-b)(ab)})		
		                         		\end{gather*} 
		                         	\end{center}                       			\[\int_{-\infty}^{\infty}p(x)dx=Re\left(\int_{-\infty}^{\infty}f(x)dx\right)= \pi  ( \frac{ae^{-kb}-be^{-ka}}{(b+a)(a-b)(ab)})\]
	When a=b, there is a double pole at ia,
	\[	 \int_{-\infty}^{\infty}f(x)dx= 2\pi i (Res_{z=ia}\frac{e^{ikz}}{(z+ia)^2(z-ia)^2} )\]
\[=2	\pi i\lim_{z\to ia} \frac{d}{dx}\frac{e^{ikz}}{(z+ia)^2}\]
	                 
\[=2	\pi i\lim_{z\to ia} \frac{-2e^{ikz}+ike^{ikz}(z+ia)}{(z+ia)^3}\]		
\[=2	\pi i \frac{-2e^{-ka}-2kae^{-ka}}{(-8ia^3)}\]
\[=	\pi \frac{e^{-ka}+kae^{-ka}}{(2a^3)}\]
	\end{enumerate} 
\end{document}